Add proofs for Classical Logic, Fix initial states

src/SequentsVLSM.v
@@ -1,20 +1,20 @@
 From Coq Require Import FunctionalExtensionality.
 From stdpp Require Import prelude.
 From VLSM.Lib Require Import ListExtras.
+From VLSM.Core Require Import VLSMProjections.
 From VLSM.Core Require Import VLSM Composition ProjectionTraces.
 From VLSM_SC Require Import Sequents.
 
 Require Import Coq.Lists.List.
 Require Import Wellfounded.
 Require Import Coq.Arith.Wf_nat.
-Require Import Coq.Arith.Lt. 
+Require Import Coq.Arith.Lt.
+ 
 
 Import Form.
 Import Calculus.
 
 (** * Sequent Calculus VLSMs *)
-
-(** This module defines the structure of sequents and the VLSMs for the identity and bottom rules of sequent calculus. *)
 
 Section sec_sequent_calculus.
 
@@ -41,9 +41,7 @@ Inductive RecEmitLeftRight : Type :=
 Inductive XCHGLabel : Type := 
 | recX
 | extract
-| exchange
-| append
-| emitX.
+| exchangeEmit.
 
 
 (** Define the structure of sequents: a pair of lists of formulas. *)
@@ -229,8 +227,8 @@ Definition V_CONJ_RIGHT_vlsm_type : VLSMType Sequent :=
 (** Transition function for the conjunction right rule. *)
 
 Definition V_CONJ_RIGHT_machine : VLSMMachine V_CONJ_RIGHT_vlsm_type :=
-  {| initial_state_prop := fun _ => True;
-     s0 := populate (exist _ None I); (* Initial state with empty Gamma and Delta *)
+  {| initial_state_prop := fun s => s = None;
+     s0 := populate (exist _ None eq_refl); (* Initial state with empty Gamma and Delta *)
      initial_message_prop := fun _ => False;
      transition := fun l '(st, msg) =>
         match l, st, msg with 
@@ -265,8 +263,8 @@ Definition V_DISJ_LEFT_vlsm_type : VLSMType Sequent :=
 
 (** Transition function for the disjunction left rule. *)
 Definition V_DISJ_LEFT_machine : VLSMMachine V_DISJ_LEFT_vlsm_type :=
-  {| initial_state_prop := fun _ => True;
-     s0 := populate (exist _ None I);
+  {| initial_state_prop := fun s => s = None;
+     s0 := populate (exist _ None eq_refl);
      initial_message_prop := fun _ => False;
      transition := fun l '(st, msg) =>
        match l, st, msg with
@@ -553,7 +551,7 @@ Definition V_XCHG_LEFT_machine : VLSMMachine V_XCHG_LEFT_vlsm_type :=
        match l, som.1, som.2 with
        | recX, ([], None), Some (seq Γ Δ) => (([], Some (seq Γ Δ)), None)
        | extract, (Γ, Some (seq (A :: Π) Δ)), None => ((Γ ++ [A], Some (seq Π Δ)), None)
-       | exchange, (Γ, Some (seq (B :: C :: Π) Δ)), None => (([], None), Some (seq (Γ ++ C :: B :: Π) Δ))
+       | exchangeEmit, (Γ, Some (seq (B :: C :: Π) Δ)), None => (([], None), Some (seq (Γ ++ C :: B :: Π) Δ))
        | _, _, _ => (([], None), None)
        end;
 
@@ -561,7 +559,7 @@ Definition V_XCHG_LEFT_machine : VLSMMachine V_XCHG_LEFT_vlsm_type :=
        match l, som.1, som.2 with
        | recX, ([], None), Some (seq Γ Δ) => True
        | extract, (Γ, Some (seq (A :: Π) Δ)), None => True
-       | exchange, (Γ, Some (seq (B :: C :: Π) Δ)), None => True
+       | exchangeEmit, (Γ, Some (seq (B :: C :: Π) Δ)), None => True
        | _, _, _ => False
        end; |}.
 
@@ -584,7 +582,7 @@ Definition V_XCHG_RIGHT_machine : VLSMMachine V_XCHG_RIGHT_vlsm_type :=
        match l, som.1, som.2 with
        | recX, ([], None), Some (seq Γ Δ) => (([], Some (seq Γ Δ)), None)
        | extract, (Γ, Some (seq Δ (A :: Π) )), None => ((Γ ++ [A], Some (seq Δ Π)), None)
-       | exchange, (Γ, Some (seq Δ (B :: C :: Π))), None => (([], None), Some (seq Δ (Γ ++ C :: B :: Π)))
+       | exchangeEmit, (Γ, Some (seq Δ (B :: C :: Π))), None => (([], None), Some (seq Δ (Γ ++ C :: B :: Π)))
        | _, _, _ => (([], None), None)
        end;
 
@@ -592,7 +590,7 @@ Definition V_XCHG_RIGHT_machine : VLSMMachine V_XCHG_RIGHT_vlsm_type :=
        match l, som.1, som.2 with
        | recX, ([], None), Some (seq Γ Δ) => True
        | extract, (Γ, Some (seq Δ (A :: Π) )), None => True
-       | exchange, (Γ, Some (seq Δ (B :: C :: Π))), None => True
+       | exchangeEmit, (Γ, Some (seq Δ (B :: C :: Π))), None => True
        | _, _, _ => False
        end;
        |}.
@@ -600,7 +598,6 @@ Definition V_XCHG_RIGHT_machine : VLSMMachine V_XCHG_RIGHT_vlsm_type :=
 Definition V_XCHG_RIGHT : VLSM Sequent := 
   mk_vlsm V_XCHG_RIGHT_machine.
 
-(*TODO: Create cutfree composition*)
 Inductive sequent_index : Type :=
 | I_V_ID
 | I_V_BOT
@@ -724,7 +721,7 @@ Lemma xchg_left_vlsm_final :
 Proof.
   intros Γ Δ Π A B.
   intros H.
-  cut (input_valid_transition sequent_vlsm (existT I_V_XCHG_LEFT exchange) 
+  cut (input_valid_transition sequent_vlsm (existT I_V_XCHG_LEFT exchangeEmit) 
           (state_update sequent_vlsm_components s0_seq I_V_XCHG_LEFT (Γ, Some (seq (A :: B :: Δ) Π)), None)
           (s0_seq, Some (seq (Γ ++ B :: A :: Δ) Π))
   ); [by eapply input_valid_transition_out |].
@@ -803,7 +800,7 @@ Lemma xchg_right_vlsm_final :
 Proof.
   intros Γ Δ Π A B.
   intros H.
-  cut (input_valid_transition sequent_vlsm (existT I_V_XCHG_RIGHT exchange) 
+  cut (input_valid_transition sequent_vlsm (existT I_V_XCHG_RIGHT exchangeEmit) 
           (state_update sequent_vlsm_components s0_seq I_V_XCHG_RIGHT (Γ, Some (seq Π (A :: B :: Δ))), None)
           (s0_seq, Some (seq Π (Γ ++ B :: A :: Δ)))
   ); [by eapply input_valid_transition_out |].
@@ -1024,6 +1021,1280 @@ Proof.
       * exfalso. by apply Hneq.
   - by apply xchg_left_vlsm_valid.
   - by apply xchg_right_vlsm_valid.
+Qed.
+
+(* Property defined on traces, meaning that all messages, input and output, represent derivable_sequents *)
+Definition trace_messages_derivable_sequents (tr : list (transition_item sequent_vlsm)): Prop :=
+  forall (m: Sequent), trace_has_message item_sends_or_receives m tr -> derivable_sequent m.
+
+Lemma elem_to_exists {A} (P : A → Prop) (x : A) (l : list A) :
+  x ∈ l → P x → Exists P l.
+Proof.
+  intros H_in H_P.
+  apply elem_of_list_In in H_in.
+  apply Exists_exists.
+  exists x.
+  split; assumption.
+Qed.
+
+
+Lemma elem_derivable_input :
+  forall (tr : list (transition_item sequent_vlsm)) (e : transition_item) (m : Sequent), 
+    e ∈ tr -> trace_messages_derivable_sequents tr
+       -> input e = Some m -> derivable_sequent m.
+Proof.
+  intros tr e m.
+  intros Hin Hder Hsome.
+  unfold trace_messages_derivable_sequents in Hder.
+  specialize (Hder m).
+  unfold trace_has_message in Hder.
+  apply Hder.
+  apply (elem_to_exists (item_sends_or_receives m) e tr Hin).
+  unfold item_sends_or_receives.
+  by left.  
+Qed.
+
+(* Helper lemma to prove that trace_messages_derivable_sequents is preserved over app*)
+Lemma trace_messages_derivable_sequents_app : 
+  forall (tr_1 tr_2 : list (transition_item sequent_vlsm)), 
+      trace_messages_derivable_sequents tr_1 ->
+      trace_messages_derivable_sequents tr_2 -> 
+        trace_messages_derivable_sequents (tr_1 ++ tr_2).
+Proof.
+  intros tr1 tr2 Htr1 Htr2.
+  intros m Hm.
+
+  apply Exists_app in Hm.
+  destruct Hm.
+  - exact (Htr1 m H).
+  - exact (Htr2 m H).
+Qed.
+  
+
+Lemma elem_of_list_split {A : Type} (x : A) (l : list A) :
+  x ∈ l -> ∃ l1 l2, l = l1 ++ x :: l2.
+Proof.
+  induction l as [| a l IH]; intros H.
+  - rewrite elem_of_nil in H. contradiction.
+  - rewrite elem_of_cons in H. destruct H as [-> | H'].
+    + exists [], l. reflexivity.
+    + destruct (IH H') as [l1 [l2 ->]]. exists (a :: l1), l2. reflexivity.
+Qed.
+
+
+Lemma input_valid_transition_in 
+  {message : Type}
+  {X : VLSM message}
+  (is s : state X)
+  (tr : list transition_item)
+  (Htrv : finite_valid_trace_init_to X is s tr)
+  (itm : transition_item)
+  (Hitm : itm ∈ tr) :
+    exists (tr_1 tr_2 : list transition_item) (lst_1 := finite_trace_last is tr_1),
+      tr = tr_1 ++ [itm] ++ tr_2 /\ input_valid_transition X (l itm) (lst_1, input itm) (destination itm, output itm).
+Proof.
+  remember (elem_of_list_split itm tr Hitm) as Hspl.
+  destruct HeqHspl, Hspl as [l1 [l2 Hspl]].
+  rewrite cons_eq_app in Hspl.
+  exists l1, l2.
+  intros.
+  split.
+  exact Hspl.
+  apply finite_valid_trace_init_to_forget_last in Htrv.
+  destruct Htrv as [Htrv _]. 
+  exact (input_valid_transition_to X is tr l1 l2 itm Htrv Hspl).
+Qed.
+
+Lemma VLSM_comp_eq: VLSM_eq {| vlsm_type := composite_type sequent_vlsm_components; vlsm_machine := free_composite_vlsm_machine sequent_vlsm_components |}
+                          (composite_vlsm sequent_vlsm_components (free_constraint sequent_vlsm_components)).
+Proof.
+  apply free_composite_vlsm_spec.
+Qed.
+
+Lemma nil_neq_app_cons : forall (A : Type) (l : list A) (x : A),
+  [] <> l ++ [x].
+Proof.
+  intros A l x H.
+  destruct l; simpl in H; discriminate.
+Qed.
+
+
+Lemma length_zero_nil : forall (A : Type) (l : list A),
+  length l = 0 -> l = [].
+Proof.
+  intros A l H.
+  destruct l as [| x xs].
+  - reflexivity.
+  - simpl in H. discriminate H.
+Qed.
+
+
+(* Helper lemma to prove that all valid traces, use as i/o only derivable sequents as messages *)
+
+Lemma all_valid_traces_derivable_sequents : 
+  forall {si sf : state sequent_vlsm} {tr : list (transition_item sequent_vlsm)}, 
+    finite_valid_trace_init_to sequent_vlsm si sf tr -> trace_messages_derivable_sequents tr.
+Proof.
+  intros si sf tr Htr.
+  (* TODO: Define an easier to use induction principle 
+           based on an assertion an all I/Os of a trace.
+  *)
+  induction Htr using finite_valid_trace_init_to_rev_strong_ind.
+  
+  intros m Hemp.
+  inversion Hemp.
+
+  (* Input should be none or derivable *)
+  assert (some_input_derivable: forall (s : Sequent), iom = Some s -> derivable_sequent s). 
+  {
+    intros s0.
+    intros Hsome.
+    subst.
+
+    unfold empty_initial_message_or_final_output in Heqiom.
+    specialize (IHHtr2 s0).
+
+    destruct (has_last_or_null iom_tr).
+    - (* iom is produced in iom_tr*)
+      destruct s1 as [l' [a Heq]].
+      apply IHHtr2.
+      rewrite Heq.
+      apply Exists_app.
+      right.
+      apply Exists_cons_hd.
+      right. 
+      exact Heqiom.
+    - (* iom_tr is empty and iom initial message -> False *)
+      destruct Heqiom as [idx [mi Hmi]].
+      destruct idx, mi, i.
+  }
+  unfold trace_messages_derivable_sequents.
+  intros m Htrapp.
+  apply Exists_app in Htrapp.
+  destruct Htrapp.
+
+  (* If the sequent comes from the prefix tr, 
+    we already know it's derivable from the induction Hypothesis *)
+
+  (* unfold trace_messages_derivable_sequents in IHHtr1. *)
+  exact (IHHtr1 m H).
+  
+  (* The remaining case is with m in the last transtion as I/O *)
+
+  inversion H; [| by inversion H1].
+  subst.
+  inversion H1; simpl in H0; subst.
+
+  (* Input of the current transition is m, we already asserted that it is derivable *)
+  subst.
+  apply (some_input_derivable m).
+  reflexivity.
+
+  (* Output, the hard case, where we have to go back through the trace. *)
+  (* To reverse the trace we should first check the label and the vlsm emiting m *)
+  destruct l as [idx lbl], idx, iom; 
+  
+  (* Unravel validity predicates *)
+  destruct Ht as [[Hv1 [Hv2 Hv3]] Htr]; 
+
+  (* Filter out invalid transitions *)
+  try by inversion Hv3.
+  - simpl in Htr.
+    injection Htr as _ Hlb.
+    subst.
+    exists 0. apply SC_ID.
+  - simpl in Htr. 
+    injection Htr as _ Hbot.
+    subst.
+    exists 0. apply SC_BOT.
+  - simpl in Htr.
+    injection Htr as _ Htop.
+    subst.
+    exists 0. apply SC_TOP.
+  - simpl in Htr.
+    destruct s0 as [L R].
+    destruct L as [| A Γ].
+    inversion Htr.
+    destruct R as [| B Δ];
+    inversion Htr.
+    subst.
+    specialize (some_input_derivable (seq (A :: Γ) (B :: Δ))).
+    cut (derivable_sequent (seq (A :: Γ) (B :: Δ)));
+      [| by apply some_input_derivable].
+    intros [h Hex].
+    exists (S h).
+    by apply SC_IMP_RIGHT.
+  - assert (Hders0: derivable_sequent s0).
+    {
+      by apply some_input_derivable.
+    }
+    destruct Hders0 as [hs0].
+    simpl in Htr.
+    destruct lbl, (s I_V_IMP_LEFT) eqn:Hse; (try by inversion Hse);
+    [| | destruct s1 as [[| B Γ'] [| A Δ]] | destruct s1 as [[| B Γ'] [|A Δ]]]; 
+      (try by inversion Hse);
+    [destruct s0 as [[| B Γ] Δ] | destruct s0 as [Γ [| A Δ]] | destruct s0 as [Γ [| A Δ]] | destruct s0 as [Γ [| A0 Δ']]| destruct s0 as [[| B Γ'] Δ']| destruct s0 as [[| B0 Γ] Δ']]; inversion Htr.
+    + cut (derivable_sequent (seq (B :: Γ') [])).
+      * intros [hr].
+        exists (S (max hs0 hr)).
+        exact (SC_IMP_LEFT A B Γ Γ' Δ [] hs0 hr H0 H2).
+      * assert (Hprev_s: exists item, 
+                        item ∈ tr /\
+                        destination item I_V_IMP_LEFT = s I_V_IMP_LEFT /\
+                        projT1 (l item) = I_V_IMP_LEFT).
+        {
+          remember (VLSM_eq_finite_valid_trace_init_to VLSM_comp_eq is s tr) as Hqq.
+          destruct HeqHqq.
+
+          destruct Hqq as [Hl1 Hr1].
+
+          remember (final_state_component_initial_or_transition I_V_IMP_LEFT is s tr (constraint := free_constraint sequent_vlsm_components) ) as Htt.
+          destruct HeqHtt.
+
+          specialize (Htt (Hl1 Htr1)).
+          destruct Htt as [Hinit | Htrans].
+          - by rewrite Hse in Hinit.
+          - destruct Htrans as [itm [Htrans1 [Htrans2 Htrans3]]].
+            by exists itm.
+        }
+        destruct Hprev_s as [itm [Hin [Hdest Hproj]]].
+        remember (l itm) as tr_lbl eqn: Heq_tr_lbl.
+        remember (destination itm) as dest_itm.
+        remember (input_valid_transition_in is s tr Htr1 itm Hin) as Htrs. 
+        destruct HeqHtrs, Htrs as [tr1 [ tr2 [Htrs Hinp]]].
+        remember (finite_trace_last is tr1) as prev_in.
+        rewrite <- Heq_tr_lbl in Hinp.
+        destruct tr_lbl as [idx lb].
+        
+        remember (input itm) as inp_itm.
+        destruct Heqdest_itm.
+        simpl in Hproj.
+        destruct Hinp as [Hval Htrans].
+        subst idx.
+        subst prev_in.
+        remember (finite_trace_last is tr1) as s0.
+        rewrite Hse in Hdest.
+        inversion Htrans as [Htrans'].
+        destruct Hval as [Hval1 [_ Hval2]]. simpl in Hval2.
+        destruct lb, (s0 I_V_IMP_LEFT); try contradiction; destruct inp_itm; try contradiction;
+        destruct s1.
+        -- destruct Gamma; try contradiction.
+           inversion Htrans' as [Hsdest].
+           pose proof (f_equal (fun h => h I_V_IMP_LEFT) Hsdest) as Himps.
+           simpl in Himps.
+           rewrite state_update_eq in Himps.
+           rewrite Hdest in Himps.
+           inversion Himps.
+           symmetry in Heqinp_itm.
+           remember (elem_derivable_input tr itm (seq (f :: Gamma) Delta) Hin IHHtr1 Heqinp_itm) as Hinp_der.
+           by rewrite <- H6, <- H7, <- H8.
+        -- destruct Delta. contradiction.
+           inversion Htrans' as [Hsdest].
+           pose proof (f_equal (fun h => h I_V_IMP_LEFT) Hsdest) as Himps.
+           simpl in Himps.
+           rewrite state_update_eq in Himps.
+           rewrite Hdest in Himps.
+           inversion Himps.
+        -- destruct Gamma. contradiction.
+           destruct s2, Delta0. contradiction.
+           inversion Htrans' as [Hsdest].
+           pose proof (f_equal (fun h => h I_V_IMP_LEFT) Hsdest) as Himps.
+           simpl in Himps.
+           rewrite state_update_eq in Himps.
+           rewrite Hdest in Himps.
+           inversion Himps.
+        -- destruct Gamma; contradiction.           
+        -- destruct Delta. contradiction.
+           destruct s2, Gamma0. contradiction.
+           inversion Htrans' as [Hsdest].
+           pose proof (f_equal (fun h => h I_V_IMP_LEFT) Hsdest) as Himps.
+           simpl in Himps.
+           rewrite state_update_eq in Himps.
+           rewrite Hdest in Himps.
+           inversion Himps.
+        -- destruct Delta; contradiction.     
+    + cut (derivable_sequent (seq (B :: Γ') (A :: Δ))); remember (A :: Δ) as Δ2.
+      * intros [hr].
+        exists (S (max hs0 hr)).
+        exact (SC_IMP_LEFT A0 B Γ Γ' Δ' Δ2 hs0 hr H0 H2).
+      * assert (Hprev_s: exists item, 
+                        item ∈ tr /\
+                        destination item I_V_IMP_LEFT = s I_V_IMP_LEFT /\
+                        projT1 (l item) = I_V_IMP_LEFT).
+        {
+          remember (VLSM_eq_finite_valid_trace_init_to VLSM_comp_eq is s tr) as Hqq.
+          destruct HeqHqq.
+
+          destruct Hqq as [Hl1 Hr1].
+
+          remember (final_state_component_initial_or_transition I_V_IMP_LEFT is s tr (constraint := free_constraint sequent_vlsm_components) ) as Htt.
+          destruct HeqHtt.
+
+          specialize (Htt (Hl1 Htr1)).
+          destruct Htt as [Hinit | Htrans].
+          - by rewrite Hse in Hinit.
+          - destruct Htrans as [itm [Htrans1 [Htrans2 Htrans3]]].
+            by exists itm.
+        }
+        destruct Hprev_s as [itm [Hin [Hdest Hproj]]].
+        remember (l itm) as tr_lbl eqn: Heq_tr_lbl.
+        remember (destination itm) as dest_itm.
+        remember (input_valid_transition_in is s tr Htr1 itm Hin) as Htrs. 
+        destruct HeqHtrs, Htrs as [tr1 [ tr2 [Htrs Hinp]]].
+        remember (finite_trace_last is tr1) as prev_in.
+        rewrite <- Heq_tr_lbl in Hinp.
+        destruct tr_lbl as [idx lb].
+        
+        remember (input itm) as inp_itm.
+        destruct Heqdest_itm.
+        simpl in Hproj.
+        destruct Hinp as [Hval Htrans].
+        subst idx.
+        subst prev_in.
+        remember (finite_trace_last is tr1) as s0.
+        rewrite Hse in Hdest.
+        inversion Htrans as [Htrans'].
+        destruct Hval as [Hval1 [_ Hval2]]. simpl in Hval2.
+        destruct lb, (s0 I_V_IMP_LEFT); try contradiction; destruct inp_itm; try contradiction; 
+        destruct s1.
+        -- destruct Gamma. contradiction.
+           inversion Htrans' as [Hsdest].
+           pose proof (f_equal (fun h => h I_V_IMP_LEFT) Hsdest) as Himps.
+           simpl in Himps.
+           rewrite state_update_eq in Himps.
+           rewrite Hdest in Himps.
+           inversion Himps.
+           symmetry in Heqinp_itm.
+           remember (elem_derivable_input tr itm (seq (f :: Gamma) Delta) Hin IHHtr1 Heqinp_itm) as Hinp_der.
+           by rewrite <- H6, <- H7, <- H8.        
+        -- destruct Delta. contradiction.
+           inversion Htrans' as [Hsdest].
+           pose proof (f_equal (fun h => h I_V_IMP_LEFT) Hsdest) as Himps.
+           simpl in Himps.
+           rewrite state_update_eq in Himps.
+           rewrite Hdest in Himps.
+           inversion Himps.
+           symmetry in Heqinp_itm.
+           subst Gamma.
+           exact (elem_derivable_input tr itm (seq (B :: Γ') (f :: Delta)) Hin IHHtr1 Heqinp_itm).
+        -- destruct Gamma. contradiction.
+           destruct s2, Delta0. contradiction.
+           inversion Htrans' as [Hsdest].
+           pose proof (f_equal (fun h => h I_V_IMP_LEFT) Hsdest) as Himps.
+           simpl in Himps.
+           rewrite state_update_eq in Himps.
+           rewrite Hdest in Himps.
+           inversion Himps.
+        -- destruct Gamma; contradiction.
+        -- destruct Delta. contradiction.
+           destruct s2, Gamma0. contradiction.
+           inversion Htrans' as [Hsdest].
+           pose proof (f_equal (fun h => h I_V_IMP_LEFT) Hsdest) as Himps.
+           simpl in Himps.
+           rewrite state_update_eq in Himps.
+           rewrite Hdest in Himps.
+           inversion Himps.  
+        -- destruct Delta; contradiction.
+    + cut (derivable_sequent (seq [] (A :: Δ))).
+      * intros [hl].
+        exists (S (max hl hs0)).
+        exact (SC_IMP_LEFT A B [] Γ' Δ Δ' hl hs0 H2 H0).
+      * assert (Hprev_s: exists item, 
+                        item ∈ tr /\
+                        destination item I_V_IMP_LEFT = s I_V_IMP_LEFT /\
+                        projT1 (l item) = I_V_IMP_LEFT).
+        {
+          remember (VLSM_eq_finite_valid_trace_init_to VLSM_comp_eq is s tr) as Hqq.
+          destruct HeqHqq.
+
+          destruct Hqq as [Hl1 Hr1].
+
+          remember (final_state_component_initial_or_transition I_V_IMP_LEFT is s tr (constraint := free_constraint sequent_vlsm_components) ) as Htt.
+          destruct HeqHtt.
+
+          specialize (Htt (Hl1 Htr1)).
+          destruct Htt as [Hinit | Htrans].
+          - by rewrite Hse in Hinit.
+          - destruct Htrans as [itm [Htrans1 [Htrans2 Htrans3]]].
+            by exists itm.
+        }
+        destruct Hprev_s as [itm [Hin [Hdest Hproj]]].
+        remember (l itm) as tr_lbl eqn: Heq_tr_lbl.
+        remember (destination itm) as dest_itm.
+        remember (input_valid_transition_in is s tr Htr1 itm Hin) as Htrs. 
+        destruct HeqHtrs, Htrs as [tr1 [ tr2 [Htrs Hinp]]].
+        remember (finite_trace_last is tr1) as prev_in.
+        rewrite <- Heq_tr_lbl in Hinp.
+        destruct tr_lbl as [idx lb].
+        
+        remember (input itm) as inp_itm.
+        destruct Heqdest_itm.
+        simpl in Hproj.
+        destruct Hinp as [Hval Htrans].
+        subst idx.
+        subst prev_in.
+        remember (finite_trace_last is tr1) as s0.
+        rewrite Hse in Hdest.
+        inversion Htrans as [Htrans'].
+        destruct Hval as [Hval1 [_ Hval2]]. simpl in Hval2.
+        destruct lb, (s0 I_V_IMP_LEFT); try contradiction; destruct inp_itm; try contradiction; 
+        destruct s1.
+        -- destruct Gamma. contradiction.
+           inversion Htrans' as [Hsdest].
+           pose proof (f_equal (fun h => h I_V_IMP_LEFT) Hsdest) as Himps.
+           simpl in Himps.
+           rewrite state_update_eq in Himps.
+           rewrite Hdest in Himps.
+           inversion Himps.
+        -- destruct Delta. contradiction.
+           inversion Htrans' as [Hsdest].
+           pose proof (f_equal (fun h => h I_V_IMP_LEFT) Hsdest) as Himps.
+           simpl in Himps.
+           rewrite state_update_eq in Himps.
+           rewrite Hdest in Himps.
+           inversion Himps.
+           symmetry in Heqinp_itm.
+           subst Gamma.
+           subst f.
+           subst Delta.
+           exact (elem_derivable_input tr itm (seq [] (A :: Δ)) Hin IHHtr1 Heqinp_itm).
+        -- destruct Gamma. contradiction.
+           destruct s2, Delta0. contradiction.
+           inversion Htrans' as [Hsdest].
+           pose proof (f_equal (fun h => h I_V_IMP_LEFT) Hsdest) as Himps.
+           simpl in Himps.
+           rewrite state_update_eq in Himps.
+           rewrite Hdest in Himps.
+           inversion Himps.
+        -- destruct Gamma; contradiction.
+        -- destruct Delta. contradiction.
+           destruct s2, Gamma0. contradiction.
+           inversion Htrans' as [Hsdest].
+           pose proof (f_equal (fun h => h I_V_IMP_LEFT) Hsdest) as Himps.
+           simpl in Himps.
+           rewrite state_update_eq in Himps.
+           rewrite Hdest in Himps.
+           inversion Himps.
+        -- destruct Delta; contradiction.
+    + cut (derivable_sequent(seq (B :: Γ') (A :: Δ))).
+      * intros [hl].
+        exists (S (max hl hs0)).
+        exact (SC_IMP_LEFT A B0 (B :: Γ') Γ Δ Δ' hl hs0 H2 H0).
+      * assert (Hprev_s: exists item, 
+                        item ∈ tr /\
+                        destination item I_V_IMP_LEFT = s I_V_IMP_LEFT /\
+                        projT1 (l item) = I_V_IMP_LEFT).
+        {
+          remember (VLSM_eq_finite_valid_trace_init_to VLSM_comp_eq is s tr) as Hqq.
+          destruct HeqHqq.
+
+          destruct Hqq as [Hl1 Hr1].
+
+          remember (final_state_component_initial_or_transition I_V_IMP_LEFT is s tr (constraint := free_constraint sequent_vlsm_components) ) as Htt.
+          destruct HeqHtt.
+
+          specialize (Htt (Hl1 Htr1)).
+          destruct Htt as [Hinit | Htrans].
+          - by rewrite Hse in Hinit.
+          - destruct Htrans as [itm [Htrans1 [Htrans2 Htrans3]]].
+            by exists itm.
+        }
+        destruct Hprev_s as [itm [Hin [Hdest Hproj]]].
+        remember (l itm) as tr_lbl eqn: Heq_tr_lbl.
+        remember (destination itm) as dest_itm.
+        remember (input_valid_transition_in is s tr Htr1 itm Hin) as Htrs. 
+        destruct HeqHtrs, Htrs as [tr1 [ tr2 [Htrs Hinp]]].
+        remember (finite_trace_last is tr1) as prev_in.
+        rewrite <- Heq_tr_lbl in Hinp.
+        destruct tr_lbl as [idx lb].
+        
+        remember (input itm) as inp_itm.
+        destruct Heqdest_itm.
+        simpl in Hproj.
+        destruct Hinp as [Hval Htrans].
+        subst idx.
+        subst prev_in.
+        remember (finite_trace_last is tr1) as s0.
+        rewrite Hse in Hdest.
+        inversion Htrans as [Htrans'].
+        destruct Hval as [Hval1 [_ Hval2]]. simpl in Hval2.
+        destruct lb, (s0 I_V_IMP_LEFT); try contradiction; destruct inp_itm; try contradiction; 
+        destruct s1.
+        -- destruct Gamma. contradiction.
+          inversion Htrans' as [Hsdest].
+          pose proof (f_equal (fun h => h I_V_IMP_LEFT) Hsdest) as Himps.
+          simpl in Himps.
+          rewrite state_update_eq in Himps.
+          rewrite Hdest in Himps.
+          inversion Himps.
+          subst f. subst Gamma. subst Delta.
+          symmetry in Heqinp_itm.
+          exact (elem_derivable_input tr itm (seq (B :: Γ') (A :: Δ)) Hin IHHtr1 Heqinp_itm).
+        -- destruct Delta. contradiction.
+           inversion Htrans' as [Hsdest].
+           pose proof (f_equal (fun h => h I_V_IMP_LEFT) Hsdest) as Himps.
+           simpl in Himps.
+           rewrite state_update_eq in Himps.
+           rewrite Hdest in Himps.
+           inversion Himps.
+           subst f. subst Gamma. subst Delta.
+           symmetry in Heqinp_itm.
+           exact (elem_derivable_input tr itm (seq (B :: Γ') (A :: Δ)) Hin IHHtr1 Heqinp_itm).
+        -- destruct Gamma. contradiction.
+           destruct s2, Delta0. contradiction.
+           inversion Htrans' as [Hsdest].
+           pose proof (f_equal (fun h => h I_V_IMP_LEFT) Hsdest) as Himps.
+           simpl in Himps.
+           rewrite state_update_eq in Himps.
+           rewrite Hdest in Himps.
+           inversion Himps.
+        -- destruct Gamma; contradiction.
+        -- destruct Delta. contradiction.
+           destruct s2, Gamma0. contradiction.
+           inversion Htrans' as [Hsdest].
+           pose proof (f_equal (fun h => h I_V_IMP_LEFT) Hsdest) as Himps.
+           simpl in Himps.
+           rewrite state_update_eq in Himps.
+           rewrite Hdest in Himps.
+           inversion Himps.
+        -- destruct Delta; contradiction.
+  - simpl in Hv3.
+    destruct lbl, (s I_V_IMP_LEFT); try contradiction; 
+    destruct s0; 
+      [by destruct Gamma | by destruct Delta].
+  - simpl in Htr.
+    destruct s0 as [L Δ].
+    destruct L as [| A Γ];
+    inversion Htr.
+    subst.
+    specialize (some_input_derivable (seq (A :: Γ) Δ)).
+    cut (derivable_sequent (seq (A :: Γ) Δ));
+      [| by apply some_input_derivable].
+    intros [h Hex].
+    exists (S h).
+    apply SC_CONJ_LEFT_1.
+    exact Hex.
+
+  - simpl in Htr.
+    destruct s0 as [L Δ].
+    destruct L as [| A Γ];
+    inversion Htr.
+    subst.
+    specialize (some_input_derivable (seq (A :: Γ) Δ)).
+    cut (derivable_sequent (seq (A :: Γ) Δ));
+      [| by apply some_input_derivable].
+    intros [h Hex].
+    exists (S h).
+    apply SC_CONJ_LEFT_2.
+    exact Hex.
+
+  - simpl in Htr.
+    destruct lbl, (s I_V_CONJ_RIGHT) eqn:Hse;
+     [by inversion Htr | | | by inversion Htr]. 
+    destruct s0, Delta; [by inversion Htr | by inversion Htr].
+
+    destruct s1 as [Γ [| A Δ]]. by inversion Htr.
+    destruct s0 as [Γ' [| B Δ']]. by inversion Htr.
+    unfold list_formula_eq in Htr.
+    destruct (decide (Γ = Γ')), (decide (Δ = Δ')); 
+    inversion Htr.
+    specialize (some_input_derivable (seq Γ' (B :: Δ'))).
+    symmetry in e, e0, H2, H3.
+    subst.
+    assert (Hdr: derivable_sequent (seq Γ (B :: Δ))). 
+    {
+      by apply some_input_derivable.
+    }
+    inversion Hdr as [hr].
+    cut (derivable_sequent (seq Γ (A :: Δ))).
+    + intros Hdl.
+      inversion Hdl as [hl].
+      exists (S (max hl hr)).
+      apply (SC_CONJ_RIGHT A B Γ Δ hl hr H2 H0).
+
+    + assert (Hprev_s: exists item, 
+                        item ∈ tr /\
+                        destination item I_V_CONJ_RIGHT = s I_V_CONJ_RIGHT /\
+                        projT1 (l item) = I_V_CONJ_RIGHT).
+      {
+        remember (VLSM_eq_finite_valid_trace_init_to VLSM_comp_eq is s tr) as Hqq.
+        destruct HeqHqq.
+
+        destruct Hqq as [Hl1 Hr1].
+        remember (final_state_component_initial_or_transition I_V_CONJ_RIGHT is s tr (constraint := free_constraint sequent_vlsm_components) ) as Htt.
+        destruct HeqHtt.
+        specialize (Htt (Hl1 Htr1)).
+        destruct Htt as [Hinit | Htrans].
+        - by rewrite Hse in Hinit.
+        - destruct Htrans as [itm [Htrans1 [Htrans2 Htrans3]]].
+          by exists itm.
+      }
+      destruct Hprev_s as [itm [Hin [Hdest Hproj]]].
+      remember (l itm) as tr_lbl eqn: Heq_tr_lbl.
+      remember (destination itm) as dest_itm.
+      remember (input_valid_transition_in is s tr Htr1 itm Hin) as Htrs. 
+      destruct HeqHtrs, Htrs as [tr1 [ tr2 [Htrs Hinp]]].
+      remember (finite_trace_last is tr1) as prev_in.
+      rewrite <- Heq_tr_lbl in Hinp.
+      destruct tr_lbl as [idx lb].
+      
+      remember (input itm) as inp_itm.
+      destruct Heqdest_itm.
+      simpl in Hproj.
+      destruct Hinp as [Hval Htrans].
+      subst idx.
+      subst prev_in.
+      remember (finite_trace_last is tr1) as s0.
+      rewrite Hse in Hdest.
+      inversion Htrans as [Htrans'].
+      destruct Hval as [Hval1 [_ Hval2]]. simpl in Hval2.
+      destruct lb eqn:Heq_lb, (s0 I_V_CONJ_RIGHT); [contradiction | | | contradiction]; 
+        [| destruct s1, Delta]; try contradiction.
+      * destruct inp_itm; [| contradiction].
+        destruct s1.
+        destruct Delta. contradiction.
+        inversion Htrans' as [Hstrans].
+        pose proof (f_equal (fun h => h I_V_CONJ_RIGHT) Hstrans) as Hsconj.
+        simpl in Hsconj.
+        rewrite state_update_eq in Hsconj.
+        rewrite Hdest in Hsconj.
+        inversion Hsconj as [Hseq].
+        symmetry in Heqinp_itm.
+        remember (elem_derivable_input tr itm (seq Gamma (f :: Delta)) Hin IHHtr1 Heqinp_itm) as Hinp_der.
+        by rewrite <- Hseq, <- H3, <- H4.
+
+      * destruct inp_itm; [| contradiction].
+        destruct s1.
+        destruct Delta0. contradiction.
+        unfold list_formula_eq in Htrans'.
+        destruct (decide (Gamma = Gamma0)), (decide (Delta = Delta0)); simpl in Htrans'; inversion Htrans' as [Hstrans];
+        pose proof (f_equal (fun h => h I_V_CONJ_RIGHT) Hstrans) as Hsconj; simpl in Hsconj; rewrite state_update_eq in Hsconj;
+        rewrite Hdest in Hsconj; by inversion Hsconj.
+
+  - simpl in Hv3.
+    destruct lbl, (s I_V_CONJ_RIGHT); try contradiction.
+    destruct s0; by destruct Delta.
+  - simpl in Htr.
+    destruct lbl, (s I_V_DISJ_LEFT) eqn:Hse;
+    [by inversion Htr | | destruct s1 as [[| A Γ] Δ]| by inversion Htr]; 
+    destruct s0 as [[| B Γ'] Δ']; 
+    try by inversion Htr.
+    unfold list_formula_eq in Htr.
+    destruct (decide (Γ = Γ')), (decide (Δ = Δ'));
+    simpl in Htr; inversion Htr.
+    specialize (some_input_derivable (seq (B :: Γ') Δ')).
+    symmetry in e, e0, H2, H3.
+    subst.
+
+    assert (Hdr: derivable_sequent (seq (B :: Γ) Δ)).
+    {
+      by apply some_input_derivable.
+    }
+
+    inversion Hdr as [hr].
+    cut (derivable_sequent(seq (A :: Γ) Δ)).
+    + intros [hl].
+      exists (S (max hl hr)).
+      apply (SC_DISJ_LEFT A B Γ Δ hl hr H2 H0).
+    + assert (Hprev_s: exists item, 
+                        item ∈ tr /\
+                        destination item I_V_DISJ_LEFT = s I_V_DISJ_LEFT /\
+                        projT1 (l item) = I_V_DISJ_LEFT).
+      {
+        remember (VLSM_eq_finite_valid_trace_init_to VLSM_comp_eq is s tr) as Hqq.
+        destruct HeqHqq.
+
+        destruct Hqq as [Hl1 Hr1].
+        remember (final_state_component_initial_or_transition I_V_DISJ_LEFT is s tr (constraint := free_constraint sequent_vlsm_components) ) as Htt.
+        destruct HeqHtt.
+        specialize (Htt (Hl1 Htr1)).
+        destruct Htt as [Hinit | Htrans].
+        - by rewrite Hse in Hinit.
+        - destruct Htrans as [itm [Htrans1 [Htrans2 Htrans3]]].
+          by exists itm.
+      }
+
+      destruct Hprev_s as [itm [Hin [Hdest Hproj]]].
+      remember (l itm) as tr_lbl eqn: Heq_tr_lbl.
+      remember (destination itm) as dest_itm.
+      remember (input_valid_transition_in is s tr Htr1 itm Hin) as Htrs. 
+      destruct HeqHtrs, Htrs as [tr1 [ tr2 [Htrs Hinp]]].
+      remember (finite_trace_last is tr1) as prev_in.
+      rewrite <- Heq_tr_lbl in Hinp.
+      destruct tr_lbl as [idx lb].
+      
+      remember (input itm) as inp_itm.
+      destruct Heqdest_itm.
+      simpl in Hproj.
+      destruct Hinp as [Hval Htrans].
+      subst idx.
+      subst prev_in.
+      remember (finite_trace_last is tr1) as s0.
+      rewrite Hse in Hdest.
+      inversion Htrans as [Htrans'].
+      destruct Hval as [Hval1 [_ Hval2]]. simpl in Hval2.
+      destruct lb, (s0 I_V_DISJ_LEFT); [contradiction | | destruct s1, Gamma | contradiction]; 
+      [ | contradiction | ]; destruct inp_itm; [| contradiction | | contradiction]; destruct s1; [destruct Gamma | destruct Gamma0];
+      try contradiction; [| (unfold list_formula_eq in *; destruct (decide (Gamma = Gamma0)), (decide (Delta = Delta0)))]; 
+      simpl in *; try contradiction; inversion Htrans'; inversion Htrans' as [Hstrans];
+      pose proof (f_equal (fun h => h I_V_DISJ_LEFT) Hstrans) as Hsdisj; simpl in Hsdisj; rewrite state_update_eq in Hsdisj;
+      rewrite Hdest in Hsdisj; inversion Hsdisj as [Hseq]. 
+      symmetry in Heqinp_itm.
+      remember (elem_derivable_input tr itm (seq (f :: Gamma) Delta) Hin IHHtr1 Heqinp_itm) as Hinp_der.
+      by rewrite <- Hseq, <- H5, <- H6.
+
+  - simpl in Hv3.
+    destruct lbl, (s I_V_DISJ_LEFT); try contradiction.
+    by destruct s0, Gamma.
+  - simpl in Htr.
+    destruct s0 as [Γ [| A Δ]];
+    inversion Htr.
+    subst.
+    specialize (some_input_derivable (seq Γ (A :: Δ))).
+    cut (derivable_sequent (seq Γ (A :: Δ)));
+      [| by apply some_input_derivable].
+    intros [h Hex].
+    exists (S h).
+    apply SC_DISJ_RIGHT_1.
+    exact Hex.
+  - simpl in Htr.
+    destruct s0 as [Γ [| A Δ]];
+    inversion Htr.
+    subst.
+    specialize (some_input_derivable (seq Γ (A :: Δ))).
+    cut (derivable_sequent (seq Γ (A :: Δ)));
+      [| by apply some_input_derivable].
+    intros [h Hex].
+    exists (S h).
+    apply SC_DISJ_RIGHT_2.
+    exact Hex.
+  - simpl in Htr.
+    destruct s0 as [Γ Δ].
+    inversion Htr.
+    subst.
+    specialize (some_input_derivable (seq Γ Δ)).
+    cut (derivable_sequent (seq Γ Δ));
+      [| by apply some_input_derivable].
+    intros [h Hex].
+    exists (S h).
+    apply SC_WK_LEFT.
+    exact Hex.
+  - simpl in Htr.
+    destruct s0 as [Γ Δ].
+    inversion Htr.
+    subst.
+    specialize (some_input_derivable (seq Γ Δ)).
+    cut (derivable_sequent (seq Γ Δ));
+      [| by apply some_input_derivable].
+    intros [h Hex].
+    exists (S h).
+    apply SC_WK_RIGHT.
+    exact Hex.
+  - simpl in Htr.
+    destruct s0 as [[| A [| B Γ]] Δ];
+    inversion Htr.
+    destruct (decide (A = B));
+    inversion H2.
+    subst.
+    specialize (some_input_derivable (seq (B :: B :: Γ) Δ)).
+    cut (derivable_sequent (seq (B :: B :: Γ) Δ));
+        [| by apply some_input_derivable].
+    intros [h Hex].
+    exists (S h).
+    apply SC_CT_LEFT.
+    exact Hex.
+  - simpl in Htr.
+    destruct s0 as [Γ [| A [| B Δ]]];
+    inversion Htr.
+    destruct (decide (A = B));
+    inversion H2.
+    subst.
+    specialize (some_input_derivable (seq Γ (B :: B :: Δ))).
+    cut (derivable_sequent (seq Γ (B :: B :: Δ)));
+        [| by apply some_input_derivable].
+    intros [h Hex].
+    exists (S h).
+    apply SC_CT_RIGHT.
+    exact Hex.
+  - simpl in Htr.
+    destruct lbl, (s I_V_XCHG_LEFT), o;
+    [destruct l | destruct l | destruct s1 | by inversion Htr | destruct s1 | by inversion Htr ]; (try by inversion Htr).
+    destruct s0. inversion Htr.
+    destruct Gamma; inversion Htr.
+    destruct Gamma. inversion Htr.
+    destruct Gamma. inversion Htr.
+    inversion Htr.
+  - simpl in Htr.
+    destruct lbl, (s I_V_XCHG_LEFT) eqn:Hse; [destruct l| | ]; (try by inversion Htr); 
+    destruct o; (try by inversion Htr); destruct s0; destruct Gamma; [| | | destruct Gamma]; try by inversion Htr.
+    inversion Htr.
+    rename l into Σ, f0 into C, f into B, Gamma into Γ, Delta into Δ.
+    assert (Hprev_s: forall is s tr Σ Γ Δ, 
+            finite_valid_trace_init_to sequent_vlsm is s tr -> s I_V_XCHG_LEFT = (Σ, Some (seq Γ Δ))
+            -> exists item, item ∈ tr /\
+                            destination item I_V_XCHG_LEFT = s I_V_XCHG_LEFT /\
+                            projT1 (l item) = I_V_XCHG_LEFT).
+    {
+      intros is0 s0 tr0 Σ0 Γ0 Δ0.
+      intros Htr0.
+      intros Hs0e.
+
+      remember (VLSM_eq_finite_valid_trace_init_to VLSM_comp_eq is0 s0 tr0) as Hqq.
+      destruct HeqHqq.
+
+      destruct Hqq as [Hl1 Hr1].
+      remember (final_state_component_initial_or_transition I_V_XCHG_LEFT is0 s0 tr0 (constraint := free_constraint sequent_vlsm_components) ) as Htt.
+      destruct HeqHtt.
+      specialize (Htt (Hl1 Htr0)).
+      destruct Htt as [Hinit | Htrans].
+      - by rewrite Hs0e in Hinit.
+      - destruct Htrans as [itm [Htrans1 [Htrans2 Htrans3]]].
+        by exists itm.
+    }
+    assert (H_prev_inv: forall is s tr Σ A Γ Δ,
+             finite_valid_trace_init_to sequent_vlsm is s tr -> s I_V_XCHG_LEFT = (Σ ++ [A], Some (seq Γ Δ))
+              -> exists item, item ∈ tr /\
+                            destination item I_V_XCHG_LEFT = (Σ, Some (seq (A :: Γ) Δ)) /\
+                            projT1 (l item) = I_V_XCHG_LEFT).
+    {
+      intros is0 s0 tr0 Σ0 A0 Γ0 Δ0.
+      intros Htr0.
+      intros Hs0e.
+      remember (Hprev_s is0 s0 tr0 (Σ0 ++ [A0]) Γ0 Δ0 Htr0 Hs0e) as Hprev.
+      destruct HeqHprev.
+      
+      destruct Hprev as [itm [Hin [Hdest Hproj]]].
+      remember (l itm) as tr_lbl eqn: Heq_tr_lbl.
+      remember (input_valid_transition_in is0 s0 tr0 Htr0 itm Hin) as Htrs. 
+      destruct HeqHtrs, Htrs as [tr1 [ tr2 [Htrs Hinp]]].
+      remember (finite_trace_last is tr1) as prev_in.
+      rewrite <- Heq_tr_lbl in Hinp.
+      destruct tr_lbl as [idx lb].
+
+      remember (input itm) as inp_itm.
+      simpl in Hproj.
+      destruct Hinp as [Hval Htrans].
+      remember (destination itm) as dest_itm.
+      subst idx.
+      subst prev_in.
+      remember (finite_trace_last is0 tr1) as s'.
+      pose proof Htr0 as Htr0'.
+      rewrite Htrs in Htr0'.
+      rewrite app_assoc in Htr0'.
+      pose proof (finite_valid_trace_init_to_prefix_1 sequent_vlsm Htr0') as Hpref.
+      unfold finite_trace_last in Hpref.
+      assert (Hlast: last (map destination (tr1 ++ [itm])) is0 = dest_itm).
+      {
+        rewrite map_app.
+        simpl.
+        by rewrite last_app.
+      }
+      rewrite Hlast in Hpref.
+      simpl in Htrans.
+      destruct Hval as [_ [_ Hval]].
+      simpl in Hval.
+
+      destruct lb, (s' I_V_XCHG_LEFT) eqn:Hs'e; [destruct l, o | destruct o | destruct o];
+      (try contradiction);
+      destruct inp_itm as [[Γ' Δ'] | ]; (try contradiction);
+      (try destruct s1);
+      (try destruct Gamma);
+      (try destruct Gamma);
+      (try contradiction);
+      injection Htrans as Htrans;
+      pose proof (f_equal (fun h => h I_V_XCHG_LEFT) Htrans) as Hloc;
+      simpl in Hloc;
+      rewrite state_update_eq in Hloc;
+      rewrite Hdest in Hloc;
+      rewrite Hs0e in Hloc;
+      inversion Hloc;
+      [by apply nil_neq_app_cons in H5 | |];
+    
+      apply app_inj_tail in H5; 
+      destruct H5 as [HlΣ HfA0];
+      subst l; subst f;
+      subst Delta; subst Γ0;
+      pose (finite_valid_trace_init_to_snoc sequent_vlsm is0 dest_itm tr1 itm) as Hvtr1;
+      apply proj1 in Hvtr1;
+      specialize (Hvtr1 Hpref);
+      rewrite <- Heqs' in Hvtr1;
+      destruct Hvtr1 as [Hvtr1 [Hvtr1' _]];
+        [pose proof (Hprev_s is0 s' tr1 Σ0 [A0] Δ0 Hvtr1 Hs'e) as Hitm_inv | pose proof (Hprev_s is0 s' tr1 Σ0 (A0 :: (f0 :: Gamma)) Δ0 Hvtr1 Hs'e) as Hitm_inv];
+      destruct Hitm_inv as [i [Hitr1 [Hidest Hiproj]]];
+      exists i; 
+        ((repeat split); [rewrite Htrs; apply elem_of_app; by left | by rewrite Hidest | exact Hiproj]).
+    }
+    assert (H_prev_capt: forall Σ is s tr  Γ Δ, 
+            finite_valid_trace_init_to sequent_vlsm is s tr -> s I_V_XCHG_LEFT = (Σ, Some (seq Γ Δ))
+            -> exists item, item ∈ tr /\
+                            destination item I_V_XCHG_LEFT = ([], Some (seq (Σ ++ Γ) Δ)) /\
+                            projT1 (l item) = I_V_XCHG_LEFT).
+    {
+      intros Σ0.
+      remember (length Σ0) as len_Σ0.
+      revert Σ0 Heqlen_Σ0.
+      induction len_Σ0.
+      - intros Σ0 Hlen is0 s0 tr0 Γ0 Δ0 Htr0 Hs0.
+        symmetry in Hlen.
+        apply length_zero_nil in Hlen.
+        subst Σ0. simpl.
+        remember (VLSM_eq_finite_valid_trace_init_to VLSM_comp_eq is0 s0 tr0) as Hqq.
+        destruct HeqHqq.
+
+        destruct Hqq as [Hl1 Hr1].
+
+        remember (final_state_component_initial_or_transition I_V_XCHG_LEFT is0 s0 tr0 (constraint := free_constraint sequent_vlsm_components) ) as Htt.
+        destruct HeqHtt.
+
+        specialize (Htt (Hl1 Htr0)).
+        destruct Htt as [Hinit | Htrans].
+        + by rewrite Hs0 in Hinit.
+        + destruct Htrans as [itm [Htrans1 [Htrans2 Htrans3]]].
+          exists itm. repeat split.
+          * auto.
+          * by rewrite Htrans2.
+          * auto.
+      - intros Σ0 Hlen is0 s0 tr0 Γ0 Δ0 HtrΣ Hs0.
+        assert (Hnotnil: Σ0 <> []).
+        {
+          destruct Σ0 as [|x xs].
+          - simpl in Hlen. discriminate Hlen.
+          - discriminate.
+        }
+        pose (exists_last Hnotnil) as Hstp.
+        destruct Hstp as [Π [A Heq]].
+        
+        subst Σ0.
+        specialize (H_prev_inv is0 s0 tr0 Π A Γ0 Δ0 HtrΣ Hs0).
+        destruct H_prev_inv as [itm [Hin [Hdst Hproj]]].
+        rewrite app_length in Hlen.
+        simpl in Hlen.
+        rewrite Nat.add_1_r in Hlen.
+        apply Nat.succ_inj in Hlen.
+        pose proof (input_valid_transition_in is0 s0 tr0 HtrΣ itm Hin) as Htrs. 
+
+        destruct Htrs as [tr1 [tr2 [Htrs Hinp]]].
+        pose proof HtrΣ as Htrp.
+        rewrite Htrs in Htrp.
+        rewrite app_assoc in Htrp.
+        pose proof (finite_valid_trace_init_to_prefix_1 sequent_vlsm Htrp) as Hpref.
+        unfold finite_trace_last in Hpref.
+        assert (Hlast: last (map destination (tr1 ++ [itm])) is0 = destination itm).
+        {
+          rewrite map_app.
+          simpl.
+          by rewrite last_app.
+        }
+        rewrite Hlast in Hpref.
+        specialize (IHlen_Σ0 Π Hlen is0 (destination itm) (tr1 ++ [itm]) (A :: Γ0) Δ0 Hpref).
+
+        specialize (IHlen_Σ0 Hdst).
+        destruct IHlen_Σ0 as [itm_res [Hin_res [Hdst_res Hproj_res]]].
+        exists itm_res. repeat split.
+        + rewrite Htrs. 
+          rewrite app_assoc.
+          apply elem_of_app.
+          by left.
+        + rewrite <- app_assoc.
+          by exact Hdst_res.
+        + exact Hproj_res.
+    }
+    cut (derivable_sequent (seq (Σ ++ B :: C :: Γ) Δ)).
+    + intros [k H_rec].
+      unfold derivable_sequent.
+      exists (S k).
+      exact (SC_XCHG_LEFT B C Σ Δ Γ k H_rec).
+    + specialize (H_prev_capt Σ is s tr (B :: C :: Γ) Δ Htr1 Hse).
+      destruct H_prev_capt as [i_capt [Hin_capt [Hdest_capt Hproj_capt]]].
+      pose proof (input_valid_transition_in is s tr Htr1 i_capt Hin_capt) as Htrs. 
+      destruct Htrs as [tr1 [tr2 [Htrs Hinp]]].
+
+      remember (destination i_capt) as dest_capt.
+      remember (input i_capt) as inp_capt.
+      remember (l i_capt) as l_capt.
+      destruct Hinp as [Hval Htrans].
+      destruct l_capt as [idx lb].
+      simpl in Hproj_capt.
+      subst idx.
+      remember (finite_trace_last is tr1) as prev_in.
+
+      simpl in Htrans.
+      simpl in Hval.
+      destruct Hval as [_ [_ Hval3]].
+      destruct lb, (prev_in I_V_XCHG_LEFT) eqn:in_eq; 
+      destruct o, l; 
+      (try contradiction);
+      destruct inp_capt as [[Γ' Δ'] | ]; (try contradiction);
+      (try destruct s0);
+      (try destruct Gamma);
+      (try destruct Gamma);
+      (try contradiction);
+      injection Htrans as Htrans;
+      pose proof (f_equal (fun h => h I_V_XCHG_LEFT) Htrans) as Hloc;
+      simpl in Hloc;
+      rewrite state_update_eq in Hloc;
+      rewrite Hdest_capt in Hloc;
+      inversion Hloc.
+      
+      subst Γ'.
+      subst Δ'.
+      symmetry in Heqinp_capt.
+      exact (elem_derivable_input tr i_capt (seq (Σ ++ B :: C :: Γ) Δ) Hin_capt IHHtr1 Heqinp_capt).
+
+  - simpl in Htr.
+    destruct lbl, (s I_V_XCHG_RIGHT); [destruct l, o | destruct o | destruct o];
+    destruct s0; (try by inversion Htr); destruct s1, Delta0; (try by inversion Htr).
+    destruct Delta0; by inversion Htr.
+  - simpl in Htr.
+    destruct lbl, (s I_V_XCHG_RIGHT) eqn:Hse; [destruct l, o| destruct o| destruct o]; (try by inversion Htr); 
+    destruct s0; destruct Delta; [| | | destruct Delta]; inversion Htr.
+    rename l into Σ, f0 into C, f into B, Gamma into Γ, Delta into Δ.
+    assert (Hprev_s: forall is s tr Σ Γ Δ, 
+            finite_valid_trace_init_to sequent_vlsm is s tr -> s I_V_XCHG_RIGHT = (Σ, Some (seq Γ Δ))
+            -> exists item, item ∈ tr /\
+                            destination item I_V_XCHG_RIGHT = s I_V_XCHG_RIGHT /\
+                            projT1 (l item) = I_V_XCHG_RIGHT).
+    {
+      intros is0 s0 tr0 Σ0 Γ0 Δ0.
+      intros Htr0.
+      intros Hs0e.
+
+      remember (VLSM_eq_finite_valid_trace_init_to VLSM_comp_eq is0 s0 tr0) as Hqq.
+      destruct HeqHqq.
+
+      destruct Hqq as [Hl1 Hr1].
+      remember (final_state_component_initial_or_transition I_V_XCHG_RIGHT is0 s0 tr0 (constraint := free_constraint sequent_vlsm_components) ) as Htt.
+      destruct HeqHtt.
+      specialize (Htt (Hl1 Htr0)).
+      destruct Htt as [Hinit | Htrans].
+      - by rewrite Hs0e in Hinit.
+      - destruct Htrans as [itm [Htrans1 [Htrans2 Htrans3]]].
+        by exists itm.
+    }
+    assert (H_prev_inv: forall is s tr Σ A Γ Δ,
+             finite_valid_trace_init_to sequent_vlsm is s tr -> s I_V_XCHG_RIGHT = (Σ ++ [A], Some (seq Γ Δ))
+              -> exists item, item ∈ tr /\
+                            destination item I_V_XCHG_RIGHT = (Σ, Some (seq Γ (A :: Δ))) /\
+                            projT1 (l item) = I_V_XCHG_RIGHT).
+    {
+      intros is0 s0 tr0 Σ0 A0 Γ0 Δ0.
+      intros Htr0.
+      intros Hs0e.
+      remember (Hprev_s is0 s0 tr0 (Σ0 ++ [A0]) Γ0 Δ0 Htr0 Hs0e) as Hprev.
+      destruct HeqHprev.
+      
+      destruct Hprev as [itm [Hin [Hdest Hproj]]].
+      remember (l itm) as tr_lbl eqn: Heq_tr_lbl.
+      remember (input_valid_transition_in is0 s0 tr0 Htr0 itm Hin) as Htrs. 
+      destruct HeqHtrs, Htrs as [tr1 [ tr2 [Htrs Hinp]]].
+      remember (finite_trace_last is tr1) as prev_in.
+      rewrite <- Heq_tr_lbl in Hinp.
+      destruct tr_lbl as [idx lb].
+
+      remember (input itm) as inp_itm.
+      simpl in Hproj.
+      destruct Hinp as [Hval Htrans].
+      remember (destination itm) as dest_itm.
+      subst idx.
+      subst prev_in.
+      remember (finite_trace_last is0 tr1) as s'.
+      pose proof Htr0 as Htr0'.
+      rewrite Htrs in Htr0'.
+      rewrite app_assoc in Htr0'.
+      pose proof (finite_valid_trace_init_to_prefix_1 sequent_vlsm Htr0') as Hpref.
+      unfold finite_trace_last in Hpref.
+      assert (Hlast: last (map destination (tr1 ++ [itm])) is0 = dest_itm).
+      {
+        rewrite map_app.
+        simpl.
+        by rewrite last_app.
+      }
+      rewrite Hlast in Hpref.
+      simpl in Htrans.
+      destruct Hval as [_ [_ Hval]].   
+      simpl in Hval.   
+      destruct lb, (s' I_V_XCHG_RIGHT) eqn:Hs'e; [destruct l, o| destruct o| destruct o]; (try contradiction);
+      destruct inp_itm; (try contradiction); destruct s1;
+      (destruct Delta); (try contradiction); (try destruct Delta); (try contradiction);
+      inversion Htrans;
+      pose proof (f_equal (fun h => h I_V_XCHG_RIGHT) H4) as Hloc;
+      simpl in Hloc;
+      rewrite state_update_eq in Hloc;
+      rewrite Hdest in Hloc;
+      rewrite Hs0e in Hloc;
+      inversion Hloc; (try by apply nil_neq_app_cons in H6);
+      apply app_inj_tail in H6;
+      destruct H6 as [HlΣ HfA0];
+      subst l; subst f; subst Gamma; subst Δ0;
+      pose (finite_valid_trace_init_to_snoc sequent_vlsm is0 dest_itm tr1 itm) as Hvtr1;
+      apply proj1 in Hvtr1;
+      specialize (Hvtr1 Hpref);
+      destruct Hvtr1 as [Hvtr1 [Hvtr1' _]];
+      rewrite <- Heqs' in Hvtr1; 
+        [pose proof (Hprev_s is0 s' tr1 Σ0 Γ0 [A0] Hvtr1 Hs'e) as Hitm_inv | pose proof (Hprev_s is0 s' tr1 Σ0 Γ0 (A0 :: (f0 :: Delta)) Hvtr1 Hs'e) as Hitm_inv];
+      destruct Hitm_inv as [i [Hitr1 [Hidest Hiproj]]];
+      exists i; 
+        ((repeat split); [rewrite Htrs; apply elem_of_app; by left | by rewrite Hidest | exact Hiproj]).
+    }
+    assert (H_prev_capt: forall Σ is s tr  Γ Δ, 
+          finite_valid_trace_init_to sequent_vlsm is s tr -> s I_V_XCHG_RIGHT = (Σ, Some (seq Γ Δ))
+          -> exists item, item ∈ tr /\
+                          destination item I_V_XCHG_RIGHT = ([], Some (seq Γ (Σ ++ Δ))) /\
+                          projT1 (l item) = I_V_XCHG_RIGHT).
+    {
+      intros Σ0.
+      remember (length Σ0) as len_Σ0.
+      revert Σ0 Heqlen_Σ0.
+      induction len_Σ0.
+      - intros Σ0 Hlen is0 s0 tr0 Γ0 Δ0 Htr0 Hs0.
+        symmetry in Hlen.
+        apply length_zero_nil in Hlen.
+        subst Σ0. simpl.
+        remember (VLSM_eq_finite_valid_trace_init_to VLSM_comp_eq is0 s0 tr0) as Hqq.
+        destruct HeqHqq.
+
+        destruct Hqq as [Hl1 Hr1].
+
+        remember (final_state_component_initial_or_transition I_V_XCHG_RIGHT is0 s0 tr0 (constraint := free_constraint sequent_vlsm_components) ) as Htt.
+        destruct HeqHtt.
+
+        specialize (Htt (Hl1 Htr0)).
+        destruct Htt as [Hinit | Htrans].
+        + by rewrite Hs0 in Hinit.
+        + destruct Htrans as [itm [Htrans1 [Htrans2 Htrans3]]].
+          exists itm. repeat split.
+          * auto.
+          * by rewrite Htrans2.
+          * auto.
+      - intros Σ0 Hlen is0 s0 tr0 Γ0 Δ0 HtrΣ Hs0.
+        assert (Hnotnil: Σ0 <> []).
+        {
+          destruct Σ0 as [|x xs].
+          - simpl in Hlen. discriminate Hlen.
+          - discriminate.
+        }
+        pose (exists_last Hnotnil) as Hstp.
+        destruct Hstp as [Π [A Heq]].
+        
+        subst Σ0.
+        specialize (H_prev_inv is0 s0 tr0 Π A Γ0 Δ0 HtrΣ Hs0).
+        destruct H_prev_inv as [itm [Hin [Hdst Hproj]]].
+        rewrite app_length in Hlen.
+        simpl in Hlen.
+        rewrite Nat.add_1_r in Hlen.
+        apply Nat.succ_inj in Hlen.
+        pose proof (input_valid_transition_in is0 s0 tr0 HtrΣ itm Hin) as Htrs. 
+
+        destruct Htrs as [tr1 [tr2 [Htrs Hinp]]].
+        pose proof HtrΣ as Htrp.
+        rewrite Htrs in Htrp.
+        rewrite app_assoc in Htrp.
+        pose proof (finite_valid_trace_init_to_prefix_1 sequent_vlsm Htrp) as Hpref.
+        unfold finite_trace_last in Hpref.
+        assert (Hlast: last (map destination (tr1 ++ [itm])) is0 = destination itm).
+        {
+          rewrite map_app.
+          simpl.
+          by rewrite last_app.
+        }
+        rewrite Hlast in Hpref.
+        specialize (IHlen_Σ0 Π Hlen is0 (destination itm) (tr1 ++ [itm]) Γ0 (A :: Δ0) Hpref).
+
+        specialize (IHlen_Σ0 Hdst).
+        destruct IHlen_Σ0 as [itm_res [Hin_res [Hdst_res Hproj_res]]].
+        exists itm_res. repeat split.
+        + rewrite Htrs. 
+          rewrite app_assoc.
+          apply elem_of_app.
+          by left.
+        + rewrite <- app_assoc.
+          by exact Hdst_res.
+        + exact Hproj_res.
+    }
+    cut (derivable_sequent (seq Γ (Σ ++ B :: C :: Δ))).
+    + intros [k H_rec].
+      unfold derivable_sequent.
+      exists (S k).
+      exact (SC_XCHG_RIGHT B C Γ Σ Δ k H_rec).
+    + specialize (H_prev_capt Σ is s tr Γ (B :: C :: Δ) Htr1 Hse).
+      destruct H_prev_capt as [i_capt [Hin_capt [Hdest_capt Hproj_capt]]].
+      pose proof (input_valid_transition_in is s tr Htr1 i_capt Hin_capt) as Htrs. 
+      destruct Htrs as [tr1 [tr2 [Htrs Hinp]]].
+
+      remember (destination i_capt) as dest_capt.
+      remember (input i_capt) as inp_capt.
+      remember (l i_capt) as l_capt.
+      destruct Hinp as [Hval Htrans].
+      destruct l_capt as [idx lb].
+      simpl in Hproj_capt.
+      subst idx.
+      remember (finite_trace_last is tr1) as prev_in.
+
+      simpl in Htrans.
+      simpl in Hval.
+      destruct Hval as [_ [_ Hval3]].
+      destruct lb, (prev_in I_V_XCHG_RIGHT) eqn:in_eq;
+      destruct o, l;
+      (try contradiction);
+      destruct inp_capt as [[Γ' Δ'] | ]; (try contradiction);
+      (try destruct s0);
+
+      (try destruct o);
+      (try destruct Delta);
+      (try destruct Delta);
+      (try contradiction);
+      injection Htrans as Htrans;
+      pose proof (f_equal (fun h => h I_V_XCHG_RIGHT) Htrans) as Hloc;
+      simpl in Hloc;
+      rewrite state_update_eq in Hloc;
+      rewrite Hdest_capt in Hloc;
+      inversion Hloc.
+      
+      subst Γ'.
+      subst Δ'.
+      symmetry in Heqinp_capt.
+      exact (elem_derivable_input tr i_capt (seq  Γ (Σ ++ B :: C :: Δ)) Hin_capt IHHtr1 Heqinp_capt).
+Qed.
+
+Theorem vlsm_valid_derivable_sequent : 
+  forall (m : Sequent), 
+    vlsm_valid_sequent (m) -> 
+      derivable_sequent(m).
+Proof.
+  intros m.
+  intros [s Hvsmp].
+  
+  apply valid_state_message_has_trace in Hvsmp as [(Hisp & H1) | (is & tr & Htr & Hout)].
+  
+  (* Initial message *)
+  - destruct H1 as [idx [mi Hmi]].
+    destruct idx, mi, i.
+
+  (* Trace *)
+  - pose proof Htr as Htr_full. 
+    destruct_list_last tr tr' lst Htr_lst;  destruct Htr as [Htr Hinit].
+    by inversion Hout.
+
+    apply finite_valid_trace_from_to_app_split in Htr as [Htr' Hlst].
+    remember (finite_trace_last is tr') as s'.
+    apply valid_trace_get_last in Hlst as Heqs.
+
+    apply valid_trace_forget_last, first_transition_valid in Hlst.
+    cbn in Heqs, Hlst; rewrite Heqs in Hlst.
+    rewrite finite_trace_last_output_is_last in Hout.
+    cut (trace_messages_derivable_sequents tr).
+    + intros Hder.
+      simpl in Hout.
+      unfold trace_messages_derivable_sequents in Hder.
+      specialize (Hder m).
+      unfold trace_has_message in Hder.
+      apply Hder.
+      rewrite Htr_lst.
+      apply Exists_app. right.
+      apply Exists_cons_hd.
+      by right. 
+    + rewrite <- Htr_lst in Htr_full.
+      exact (all_valid_traces_derivable_sequents Htr_full). 
 Qed.
 
 End sec_sequent_calculus.
